backend/ValueAnalysis.v
@@ -2041,7 +2041,7 @@ Proof.
     + red. intros. apply valid_pmatch in H. eauto.
   - apply bc_of_se_mem_nostack.
   - admit.
-Admitted.
+Abort.
 
 End BCgen.
 
