cklr/VAInject.v
@@ -400,7 +400,7 @@ Proof.
     + exists (injw f' (Mem.support m1') (Mem.support m2')).
       repeat apply  conj; econstructor; eauto.
       constructor; eauto.
-Admitted.
+Abort.
       
     
   
